theories/elpi_test.v
@@ -384,7 +384,7 @@ Goal forall l,
   let s := ((Or (Or Dead empty (CutS)) empty OK)) in
   let bt := of_alt([::] :: l) in
   t2l s empty (of_alt l) = of_alt[:: [:: cut bt]; [::]] /\ 
-    t2l (odflt Bot (next_alt true (get_tree (expand u empty s)))) empty (of_alt l) ++ (of_alt l) = bt.
+    t2l (odflt Bot (next_alt true (get_tree (step u empty s)))) empty (of_alt l) ++ (of_alt l) = bt.
 Proof.
   simpl get_tree.
   move=>//=.
